wip

Matroid/Constructions/Truncate.lean
@@ -199,10 +199,9 @@ lemma circuit_iff_restr_eq_circuitOn (hCne : C.Nonempty) (hC : C ⊆ M.E := by a
 
 end circuitOn
 
-section Local
+section Partial
 
-variable {I J B : Set α} {Bs : Set (Set α)}
-
+variable {I J B B' : Set α} {e f : α}
 
 lemma Base.base_of_indep_of_finDiff (hB : M.Base B) (hI : M.Indep I) (hBI : FinDiff B I) :
     M.Base I := by
@@ -212,15 +211,234 @@ lemma Base.base_of_indep_of_finDiff (hB : M.Base B) (hI : M.Indep I) (hBI : FinD
     exact hBI.diff_left_finite.subset (diff_subset_diff_right hIB')
   rwa [(hBI.symm.trans hfin').eq_of_subset hIB']
 
-def LocalTruncateIndep (M : Matroid α) (Bs : Set (Set α)) (I : Set α) : Prop := M.Indep I ∧ I ∉ Bs
+@[ext] structure PartialTruncateCollection (M : Matroid α) where
+  ToTruncate : Set α → Prop
+  forall_nonempty : ∀ ⦃B⦄, ToTruncate B → B.Nonempty
+  forall_base : ∀ ⦃B⦄, ToTruncate B → M.Base B
+  toTruncate_of_toTruncate : ∀ ⦃B B' e e'⦄, ToTruncate B → e ∈ B → M.Base B' → e' ∈ B' →
+      M.closure (B \ {e}) = M.closure (B' \ {e'}) → ToTruncate B'
 
-lemma LocalTruncateIndep.subset (hI : M.LocalTruncateIndep Bs I) (hBs : ∀ ⦃B⦄, B ∈ Bs → M.Base B)
-    (hJI : J ⊆ I) : M.LocalTruncateIndep Bs J :=
-  ⟨hI.1.subset hJI, fun hJBs ↦ hI.2 <| by rwa [← (hBs hJBs).eq_of_subset_indep hI.1 hJI] ⟩
+variable {T : M.PartialTruncateCollection}
 
-lemma maximal_localTruncateIndep_iff (hBs_base : ∀ ⦃B⦄, B ∈ Bs → M.Base B)
-    (hBs_finDiff : ∀ ⦃B B'⦄, B ∈ Bs → M.Base B' → FinDiff B B' → B' ∈ Bs) :
-    Maximal (M.LocalTruncateIndep Bs) B ↔ (M.Base B ∧ B ∉ Bs) ∨ (∃ e ∉ B, insert e B ∈ Bs) := by
+lemma PartialTruncateCollection.ToTruncate.base (hB : T.ToTruncate B) : M.Base B :=
+  T.forall_base hB
+
+lemma PartialTruncateCollection.ToTruncate.nonempty (hB : T.ToTruncate B) : B.Nonempty :=
+  T.forall_nonempty hB
+
+
+lemma PartialTruncateCollection.ToTruncate.toTruncate_of_closure (hI : T.ToTruncate (insert e I))
+    (heI : e ∉ I) (hfJ : f ∉ J) (hJ : M.Indep (insert f J)) (hIJ : I ⊆ M.closure J) :
+    T.ToTruncate (insert f J) := by
+  have hhp : M.Hyperplane (M.closure I) := by
+    simpa [heI] using hI.base.hyperplane_of_closure_diff_singleton (mem_insert _ _)
+  replace hJ := show M.Base (insert f J) by
+    refine hJ.base_of_ground_subset_closure ?_
+    have hssu : M.closure I ⊂ M.closure (insert f J) := by
+      refine (M.closure_subset_closure_of_subset_closure hIJ).trans_ssubset ?_
+      exact hJ.closure_ssubset_closure (ssubset_insert hfJ)
+    rw [← hhp.closure_eq_ground_of_ssuperset hssu, closure_closure]
+  refine T.toTruncate_of_toTruncate hI (mem_insert _ _) hJ (mem_insert _ _) ?_
+
+  suffices hJI : J ⊆ M.closure I by simp [(M.closure_subset_closure_of_subset_closure hIJ).antisymm
+    (M.closure_subset_closure_of_subset_closure hJI), heI, hfJ]
+  have hJE := (subset_insert _ _).trans hJ.subset_ground
+  refine fun x hxJ ↦ by_contra fun hxI ↦ ?_
+  have hcl := (hhp.closure_insert_eq_univ ⟨hJE hxJ, hxI⟩).symm.subset
+  rw [closure_insert_closure_eq_closure_insert] at hcl
+  replace hcl := hcl.trans (M.closure_subset_closure (insert_subset_insert hIJ))
+  rw [closure_insert_closure_eq_closure_insert, insert_eq_of_mem hxJ] at hcl
+  have hcl' := hJ.indep.closure_diff_singleton_ssubset (mem_insert _ _)
+  simp only [mem_singleton_iff, insert_diff_of_mem, hfJ, not_false_eq_true,
+    diff_singleton_eq_self, hJ.closure_eq] at hcl'
+  exact hcl'.not_subset hcl
+
+lemma PartialTruncateCollection.ToTruncate.exchange (hB : T.ToTruncate B) (heB : e ∉ B)
+    (hfB : f ∈ B) (h_base : M.Base (insert e (B \ {f}))) : T.ToTruncate (insert e (B \ {f})) := by
+  have hef : e ≠ f := by rintro rfl; contradiction
+  exact T.toTruncate_of_toTruncate hB hfB h_base (mem_insert _ _)
+    <| by simp [diff_singleton_eq_self (show e ∉ B \ {f} by simp [heB, hef])]
+
+lemma PartialTruncateCollection.ToTruncate.of_exchange (hB' : T.ToTruncate (insert e (B \ {f})))
+    (heB : e ∉ B) (hfB : f ∈ B) (hB : M.Base B) : T.ToTruncate B := by
+  have hef : e ≠ f := by rintro rfl; contradiction
+  have hrw : B = insert f (insert e (B \ {f}) \ {e}) := by
+    simp [diff_singleton_eq_self (show e ∉ B \ {f} by simp [hef, heB]), insert_eq_of_mem hfB]
+  rw [hrw]
+  exact hB'.exchange (by simp [hef.symm]) (mem_insert _ _) <| (by rwa [← hrw])
+
+lemma PartialTruncateCollection.ToTruncate.finDiff {B B' : Set α} (hB : T.ToTruncate B)
+    (hB' : M.Base B') (hdiff : FinDiff B B') : T.ToTruncate B' := by
+  obtain h | h := (B \ B').eq_empty_or_nonempty
+  · rw [diff_eq_empty] at h
+    rwa [← hB.base.eq_of_subset_base hB' h]
+  obtain ⟨f, hf⟩ := hdiff.symm.nonempty_of_nonempty h
+  obtain ⟨e, he, heB⟩ := hB'.exchange hB.base hf
+  have hlt : ((insert e (B' \ {f})) \ B).encard < (B' \ B).encard := by
+    rw [insert_diff_of_mem _ he.1, diff_diff_comm, ← encard_diff_singleton_add_one hf,
+      ENat.lt_add_one_iff]
+    simpa using hdiff.diff_right_finite.diff {f}
+  have hfd : FinDiff B (insert e (B' \ {f})) := hdiff.trans (finDiff_exchange hf.1 he.2)
+  exact (PartialTruncateCollection.ToTruncate.finDiff hB heB hfd).of_exchange he.2 hf.1 hB'
+termination_by (B' \ B).encard
+
+def PartialTruncateCollection.Indep (T : M.PartialTruncateCollection) (I : Set α) : Prop :=
+  M.Indep I ∧ ¬ T.ToTruncate I
+
+def PartialTruncateCollection.Base (T : M.PartialTruncateCollection) (B : Set α) : Prop :=
+  (M.Base B ∧ ¬ T.ToTruncate B) ∨ (∃ e ∈ M.E \ B, T.ToTruncate (insert e B))
+
+lemma PartialTruncateCollection.ToTruncate.base_diff_singleton (hBt : T.ToTruncate B)
+    (heB : e ∈ B) : T.Base (B \ {e}) :=
+  .inr ⟨e, by simpa [hBt.base.subset_ground heB, heB] ⟩
+
+lemma PartialTruncateCollection.ToTruncate.base_of_insert (hBt : T.ToTruncate (insert e B))
+  (heB : e ∉ B) : T.Base B := sorry
+
+lemma PartialTruncateCollection.ToTruncate.not_base (hBt : T.ToTruncate B) : ¬ T.Base B := by
+  sorry
+
+lemma PartialTruncateCollection.Base.indep (hB : T.Base B) : T.Indep B := by
+  obtain h | ⟨e, he, heB⟩ := hB
+  · exact ⟨h.1.indep, h.2⟩
+  refine ⟨heB.base.indep.subset <| subset_insert _ _, fun hBt ↦ ?_⟩
+  rw [hBt.base.eq_of_subset_base heB.base (subset_insert _ _)] at he
+  simp at he
+
+-- lemma PartialTruncateCollection.Base.base_insert (hB : T.Base B) (hBM : ¬ M.Base B)
+--     (he : e ∈ M.E \ B) : M.Base (insert e B) := sorry
+
+-- lemma PartialTruncateCollection.Base.exists_base_insert (hB : T.Base B) (hBM : ¬ M.Base B) :
+--     ∃ e ∈ M.E \ B, T.ToTruncate (insert e B) := by
+--   rw [PartialTruncateCollection.Base, iff_false_intro hBM] at hB
+
+lemma PartialTruncateCollection.Base.exists_toTruncate_insert (hB : T.Base B) (hBM : ¬ M.Base B) :
+    ∃ e ∈ M.E \ B, T.ToTruncate (insert e B) := sorry
+
+lemma PartialTruncateCollection.Base.toTruncate_insert (hB : T.Base B) (hBM : ¬ M.Base B)
+    (he : e ∈ M.E \ B) : T.ToTruncate (insert e B) := sorry
+
+
+
+lemma PartialTruncateCollection.Indep.indep (hI : T.Indep I) : M.Indep I :=
+  hI.1
+
+lemma Base.partialTruncateBase_iff (hB : M.Base B) : T.Base B ↔ ¬ T.ToTruncate B := sorry
+
+lemma Base.partialTruncateBase (hB : M.Base B) (hBt : ¬ T.ToTruncate B) : T.Base B :=
+  .inl ⟨hB, hBt⟩
+
+lemma PartialTruncateCollection.Indep.subset (hI : T.Indep I) (hJI : J ⊆ I) : T.Indep J :=
+  ⟨hI.1.subset hJI, fun hT ↦ hI.2 <| by rwa [← hT.base.eq_of_subset_indep hI.indep hJI]⟩
+
+lemma PartialTruncateCollection.indep_iff_subset_base : T.Indep I ↔ ∃ B, T.Base B ∧ I ⊆ B := by
+  constructor
+  · rintro ⟨hI, hIt⟩
+    obtain ⟨B, hB, hIB⟩ := hI.exists_base_superset
+    by_cases hBt : T.ToTruncate B
+    · obtain ⟨e, he⟩ := exists_of_ssubset (hIB.ssubset_of_ne <| by rintro rfl; contradiction)
+      exact ⟨B \ {e}, hBt.base_diff_singleton he.1, subset_diff_singleton hIB he.2⟩
+    refine ⟨B, .inl ⟨hB, hBt⟩, hIB⟩
+  rintro ⟨B, hB |⟨e, he, heB⟩, hIB⟩
+  · exact ⟨hB.1.indep.subset hIB, fun hI ↦ hB.2 <| by rwa [← hI.base.eq_of_subset_base hB.1 hIB]⟩
+  exact (heB.base_diff_singleton (mem_insert _ _)).indep.subset <|
+    by simpa [diff_singleton_eq_self he.2]
+
+lemma maximal_localTruncateIndep_eq : Maximal (T.Indep) = T.Base := by
+  ext B
+  sorry
+  -- refine ⟨fun h ↦ ?_, fun h ↦ ?_⟩
+  -- ·
+
+def PartialTruncateCollection.indepMatroid (T : M.PartialTruncateCollection) : IndepMatroid α where
+  E := M.E
+  Indep := T.Indep
+  indep_empty := sorry
+  indep_subset := sorry
+  indep_aug := by
+    simp_rw [maximal_localTruncateIndep_eq]
+    intro I B ⟨hI, hIt⟩ hItb hB
+    have hInotbase : ¬ M.Base I := fun hIb ↦ hItb (.inl ⟨hIb, hIt⟩)
+
+    by_cases hBM : M.Base B
+    · obtain ⟨e, heBI, heI⟩ := hI.exists_insert_of_not_base hInotbase hBM
+      refine ⟨e, heBI, heI, fun heIt ↦ hItb ?_⟩
+      simpa [heBI.2] using heIt.base_diff_singleton <| mem_insert _ _
+    by_cases hcon : B ⊆ M.closure I
+    · obtain ⟨e, he, heB⟩ := hB.exists_toTruncate_insert hBM
+      have := heB.toTruncate_of_closure he.2 (J := I) (f := e)
+
+    simp only [subset_def, not_forall, Classical.not_imp, exists_prop] at hcon
+    obtain ⟨e, heB, he⟩ := hcon
+    have heI : e ∉ I := not_mem_subset (M.subset_closure _) he
+    rw [hI.not_mem_closure_iff_of_not_mem heI (hB.indep.indep.subset_ground heB)] at he
+    exact ⟨e, ⟨heB, heI⟩, he, fun hT ↦ hItb (hT.base_of_insert heI)⟩
+
+
+    -- obtain ⟨e, he, heB⟩ := hB.exists_toTruncate_insert hBM
+
+
+
+
+      -- have := hI.exists_insert_of_not_base
+  indep_maximal := sorry
+  subset_ground := sorry
+
+
+-- def PartialTruncateCollection.indepMatroid (T : M.PartialTruncateCollection) : Matroid α where
+--   E := M.E
+--   Base := T.Base
+--   Indep := T.Indep
+--   indep_iff' _ := indep_iff_subset_base
+--   exists_base := by
+--     obtain ⟨B, hB⟩ := M.exists_base
+--     by_cases hBt : T.ToTruncate B
+--     · obtain ⟨e, he⟩ := hBt.nonempty
+--       exact ⟨_, hBt.base_diff_singleton he⟩
+--     exact ⟨B, hB.partialTruncateBase hBt⟩
+--   base_exchange := by
+--     rintro B B' hB hB' e he
+--     by_cases hBM : M.Base B
+
+--     -- rw [Base.partialTruncateBase]
+--     · by_cases hB'M : M.Base B'
+--       · obtain ⟨f, hf, hfB⟩ := hBM.exchange hB'M he
+--         exact ⟨f, hf, hfB.partialTruncateBase fun h ↦ (h.of_exchange hf.2 he.1 hBM).not_base hB⟩
+--       by_contra! hcon
+
+--       have hBeM := hB'.toTruncate_insert hB'M ⟨hBM.subset_ground he.1, he.2⟩
+
+--       have hcon' := hBeM.toTruncate_of_closure (e := e) (f := e) (J := B \ {e}) he.2
+--         (hBM.indep.subset diff_subset) ?_ (by simp)
+--       · simp only [insert_diff_singleton, he.1, insert_eq_of_mem] at hcon'
+--         exact hcon'.not_base hB
+--       rw []
+
+
+      -- rw [PartialTruncateCollection.Base, iff_false_intro hB'M, false_and, false_or] at hB'
+
+
+
+    -- by_cases hBt : T.ToTruncate B
+    -- · by_cases hBt' : T.ToTruncate B'
+    --   ·
+    --     -- obtain ⟨f, hf⟩ : (B' \ B).Nonempty := sorry
+    --     obtain ⟨f, hf, hBf⟩ := hBt.base.exchange hBt'.base he
+
+    --     refine ⟨f, hf, ?_⟩
+
+        -- have := (hBt.base_diff_singleton he.1).exchange (hBt'.base_diff_singleton hf.1)
+
+
+
+  --   sorry
+
+
+  -- maximality := _
+  -- subset_ground := _
+
+lemma maximal_localTruncateIndep_eq : Maximal (T.Indep) = T.Base := by
+  ext
   rw [maximal_subset_iff, LocalTruncateIndep]
   refine ⟨fun ⟨⟨hBi, hBb⟩, hmax⟩ ↦ ?_, ?_⟩
   · obtain ⟨B', hB', hBB'⟩ := hBi.exists_base_superset
@@ -228,22 +446,22 @@ lemma maximal_localTruncateIndep_iff (hBs_base : ∀ ⦃B⦄, B ∈ Bs → M.Bas
     · exact .inl ⟨hB', hBb⟩
     right
     obtain ⟨e, heB', heB⟩ := exists_of_ssubset hss
-    refine ⟨e, heB, by_contra fun heBb ↦ ?_⟩
+    refine ⟨e, ⟨hB'.subset_ground heB', heB⟩, by_contra fun heBb ↦ ?_⟩
     rw [hmax ⟨(hB'.indep.subset (insert_subset heB' hBB')), heBb⟩ (subset_insert _ _)] at heB
     simp at heB
   rintro (⟨hB, hBb⟩ | ⟨e, heB, heBb⟩)
   · exact ⟨⟨hB.indep, hBb⟩, fun J hJ hBJ ↦ hB.eq_of_subset_indep hJ.1 hBJ⟩
-  refine ⟨⟨?_, fun hBs ↦ heB ?_⟩, fun J hJ hBJ ↦ by_contra fun hne ↦ ?_⟩
-  · exact (hBs_base heBb).indep.subset (subset_insert _ _)
-  · rw [(hBs_base hBs).eq_of_subset_base (hBs_base heBb) (subset_insert _ _)]
+  refine ⟨⟨?_, fun hT ↦ heB.2 ?_⟩, fun J hJ hBJ ↦ by_contra fun hne ↦ ?_⟩
+  · exact (hT_base heBb).indep.subset (subset_insert _ _)
+  · rw [(hT_base hT).eq_of_subset_base (hT_base heBb) (subset_insert _ _)]
     simp
   obtain ⟨f, hfJ, hfB⟩ := exists_of_ssubset (hBJ.ssubset_of_ne hne)
 
   have hfB_base : M.Base (insert f B) :=
-    (hBs_base heBb).base_of_indep_of_finDiff (hJ.1.subset (insert_subset hfJ hBJ))
+    (hT_base heBb).base_of_indep_of_finDiff (hJ.1.subset (insert_subset hfJ hBJ))
     (finDiff_insert_insert heB hfB)
   obtain rfl : insert f B = J := hfB_base.eq_of_subset_indep hJ.1 (insert_subset hfJ hBJ)
-  exact hJ.2 <| hBs_finDiff heBb hfB_base (finDiff_insert_insert heB hfB)
+  exact hJ.2 <| hT_finDiff heBb hfB_base (finDiff_insert_insert heB hfB)
 
 
 
@@ -252,16 +470,16 @@ For finite uniform matroids, this just reduces the rank by one. For infinite one
 This is weird, since it forms a proper quotient that still has a common base with `M` -/
 
 
--- def LocalTruncateIndepMatroid (M : Matroid α) (hr : M.RkPos) (Bs : Set (Set α))
---     (hBs_base : ∀ ⦃B⦄, B ∈ Bs → M.Base B)
---     (hBs_finDiff : ∀ ⦃B B'⦄, B ∈ Bs → M.Base B' → FinDiff B B' → B' ∈ Bs) : IndepMatroid α where
+-- def LocalTruncateIndepMatroid (M : Matroid α) (hr : M.RkPos) (T : Set (Set α))
+--     (hT_base : ∀ ⦃B⦄, B ∈ T → M.Base B)
+--     (hT_finDiff : ∀ ⦃B B'⦄, B ∈ T → M.Base B' → FinDiff B B' → B' ∈ T) : IndepMatroid α where
 --   E := M.E
---   Indep := M.LocalTruncateIndep Bs
---   indep_empty := ⟨M.empty_indep, fun h ↦ M.empty_not_base (hBs_base h)⟩
+--   Indep := M.LocalTruncateIndep T
+--   indep_empty := ⟨M.empty_indep, fun h ↦ M.empty_not_base (hT_base h)⟩
 
---   indep_subset I J hJ hIJ := hJ.subset hBs_base hIJ
+--   indep_subset I J hJ hIJ := hJ.subset hT_base hIJ
 --   indep_aug := by
---     simp only [maximal_localTruncateIndep_iff hBs_base hBs_finDiff, not_or, not_and, not_not,
+--     simp only [maximal_localTruncateIndep_iff hT_base hT_finDiff, not_or, not_and, not_not,
 --       not_exists, mem_diff, and_imp]
 --     rintro I B hI hInotbase hBmax
 --     replace hInotbase := show ¬ M.Base I by simpa [hI.2] using hInotbase
@@ -271,23 +489,23 @@ This is weird, since it forms a proper quotient that still has a common base wit
 --     -- have heI : e ∈ I := by
 --     --   by_contra heI
 --     --   have := hBmax _ heI
---     obtain ⟨f, ⟨(rfl | hf), hfI⟩, hfi⟩ := hI.1.exists_insert_of_not_base hInotbase (hBs_base heBb)
+--     obtain ⟨f, ⟨(rfl | hf), hfI⟩, hfi⟩ := hI.1.exists_insert_of_not_base hInotbase (hT_base heBb)
 --     ·
 --       by_cases hbase : M.Base (insert f I)
 --       · sorry
---       obtain ⟨g, hg, hgi⟩ := hfi.exists_insert_of_not_base hbase (hBs_base heBb)
+--       obtain ⟨g, hg, hgi⟩ := hfi.exists_insert_of_not_base hbase (hT_base heBb)
 --       simp only [mem_insert_iff, true_or, insert_diff_of_mem, mem_diff, not_or] at hg
 --       rw [insert_comm] at hgi
 --       refine ⟨g, ⟨hg.1, hg.2.2⟩, hgi.subset (subset_insert _ _), fun hgI ↦ ?_⟩
 --       obtain (rfl | hfI) : f ∈ insert g I :=
---         ((hBs_base hgI).eq_of_subset_indep hgi (subset_insert _ _)).symm.subset (mem_insert f _)
+--         ((hT_base hgI).eq_of_subset_indep hgi (subset_insert _ _)).symm.subset (mem_insert f _)
 --       · exact hg.2.1 rfl
 --       contradiction
---       --   -- have := hbase.exchange (hBs_base heBb) (e := f)
+--       --   -- have := hbase.exchange (hT_base heBb) (e := f)
 
 --       -- sorry
 --     sorry
-        -- have := hbase.exchange (hBs_base heBb)
+        -- have := hbase.exchange (hT_base heBb)
 
 
 
@@ -298,14 +516,14 @@ This is weird, since it forms a proper quotient that still has a common base wit
     -- by_cases hB : M.Base B
     -- · obtain ⟨e, heBI, heI⟩ := hI.1.exists_insert_of_not_base hInotbase hB
     --   obtain ⟨f, hfI, hins⟩ :=
-    --     exists_insert_of_not_maximal (fun I J hJ hIJ ↦ hJ.subset hBs_base hIJ) hI hInotmax
-    --   refine ⟨e, heBI, heI, fun heIBs ↦ hins.2 ?_⟩
-    --   refine hBs_finDiff heIBs ?_ (finDiff_insert_insert heBI.2 hfI)
-    --   exact (hBs_base heIBs).base_of_indep_of_finDiff hins.1 (finDiff_insert_insert heBI.2 hfI)
+    --     exists_insert_of_not_maximal (fun I J hJ hIJ ↦ hJ.subset hT_base hIJ) hI hInotmax
+    --   refine ⟨e, heBI, heI, fun heIT ↦ hins.2 ?_⟩
+    --   refine hT_finDiff heIT ?_ (finDiff_insert_insert heBI.2 hfI)
+    --   exact (hT_base heIT).base_of_indep_of_finDiff hins.1 (finDiff_insert_insert heBI.2 hfI)
 
     -- obtain ⟨B₀, hB₀⟩ := M.exists_base
     -- obtain ⟨e, ⟨-, heB⟩, heBi⟩ := hBmax.prop.1.exists_insert_of_not_base hB hB₀
-    -- have heBb : insert e B ∈ Bs :=
+    -- have heBb : insert e B ∈ T :=
     --   by_contra fun h' ↦ hBmax.not_prop_of_ssuperset (ssubset_insert heB) ⟨heBi, h'⟩
     -- have :=
 
